tarski wip

SmullyanSystem/Basic.lean
@@ -39,9 +39,26 @@ structure Sentence (M : SmullyanModel) where
   P : M.Predicate
   W : M.Word
 
+lemma Sentence.ext : ∀ {S₁ S₂ : M.Sentence}, S₁.P = S₂.P → S₁.W = S₂.W → S₁ = S₂ := by
+  intros S₁ S₂ hP hW;
+  cases S₁; cases S₂;
+  subst hP hW;
+  tauto;
+
 abbrev sentences (M : SmullyanModel) : Set M.Sentence := Set.univ
 
 def Sentence.toWord : M.Sentence → M.Word := fun ⟨P, W⟩ => P ++ W
+
+lemma Sentence.exists_unique (S : M.Sentence) : ∃! P, ∃! W, ⟨P, W⟩ = S := by sorry;
+
+@[simp]
+lemma Sentence.toWord_injective : Function.Injective (Sentence.toWord (M := M)) := by
+  simp [Function.Injective, Sentence.toWord];
+  intro S₁ S₂ h;
+  obtain ⟨P₁, ⟨W₁, rfl, hW₁⟩, hP₁⟩ := Sentence.exists_unique S₁;
+  obtain ⟨P₂, ⟨W₂, rfl, hW₂⟩, hP₂⟩ := Sentence.exists_unique S₂;
+  sorry;
+
 
 instance : Coe (M.Sentence) (M.Word) := ⟨Sentence.toWord⟩
 
@@ -63,20 +80,27 @@ abbrev proper_sentences (M : SmullyanModel) : Set M.ProperSentence := Set.univ
 def isProperSentence (W : M.Word) : Prop := M.isSentence W ∧ ¬M.isPredicate W
 
 
-def true_sentences (M : SmullyanModel) : Set M.Sentence := fun ⟨P, W⟩ => W ∈ P.valuated
+abbrev true_sentences (M : SmullyanModel) : Set M.Sentence := fun ⟨P, W⟩ => W ∈ P.valuated
 
-def true_proper_sentences (M : SmullyanModel) : Set M.ProperSentence := fun ⟨⟨P, W⟩, _⟩ => W ∈ M.valuation P
+abbrev true_proper_sentences (M : SmullyanModel) : Set M.ProperSentence := fun ⟨⟨P, W⟩, _⟩ => W ∈ M.valuation P
 
-def false_sentences (M : SmullyanModel) : Set M.Sentence := M.sentences \ M.true_sentences
+abbrev false_sentences (M : SmullyanModel) : Set M.Sentence := M.true_sentencesᶜ
 
-def false_proper_sentences (M : SmullyanModel) : Set M.ProperSentence := M.proper_sentences \ M.true_proper_sentences
+abbrev false_proper_sentences (M : SmullyanModel) : Set M.ProperSentence := M.true_proper_sentencesᶜ
 
 
 def Sentence.isTrue (S : M.Sentence) := S ∈ M.true_sentences
 prefix:90 "⊨ " => Sentence.isTrue
 
-@[simp] lemma iff_mem_true_sentences : ⊨ S ↔ S.W ∈ S.P.valuated := by rfl
+lemma Sentence.iff_isTrue : ⊨ S ↔ S.W ∈ S.P.valuated := by rfl
 
+
+def Sentence.isFalse (S : M.Sentence) := S ∈ M.false_sentences
+prefix:90 "⊭ " => Sentence.isFalse
+
+lemma Sentence.iff_isFalse_not_isTrue : ⊭ S ↔ ¬⊨ S := by simp [false_sentences, Sentence.isTrue, Sentence.isFalse]
+
+lemma Sentence.iff_isFalse : ⊭ S ↔ S.W ∉ S.P.valuated := by simp [iff_isTrue, iff_isFalse_not_isTrue]
 
 
 class IsN (M : SmullyanModel) where
@@ -95,7 +119,6 @@ def Sentence.negated (S : M.Sentence) : M.Sentence := ⟨~S.P, S.W⟩
 prefix:90 "~" => Sentence.negated
 
 def Sentence.isNegTrue (S : M.Sentence) := ⊨ ~S
-prefix:50 "⊭ " => Sentence.isNegTrue
 
 @[simp]
 lemma iff_negated_valuated {P : M.Predicate} : (~P).valuated = P.valuatedᶜ := by
@@ -133,16 +156,51 @@ variable {P : M.Predicate} {S : M.Sentence}
 
 def Predicate.fixpoint [M.IsR] (P : M.Predicate) : M.Sentence := ⟨□P, □P⟩
 
-lemma fixpoint_spec [M.IsR] : ⊨ P.fixpoint ↔ ⊨ (⟨P, P.fixpoint⟩) := by simp [Predicate.fixpoint];
+lemma fixpoint_spec [M.IsR] : ⊨ P.fixpoint ↔ ⊨ (⟨P, P.fixpoint⟩) := by
+  simp [Predicate.fixpoint, Sentence.iff_isTrue];
 
-lemma iff_fixpoint_is_true [M.IsNR] : ⊨ (~P).fixpoint ↔ ↑(~P).fixpoint ∉ P.valuated := by simp [Predicate.fixpoint];
+lemma iff_fixpoint_is_true [M.IsNR] : ⊨ (~P).fixpoint ↔ ↑(~P).fixpoint ∉ P.valuated := by
+  simp [Predicate.fixpoint, Sentence.iff_isTrue];
 
-theorem tarski [M.IsNR] : ¬∃ P : M.Predicate, P.names M.true_sentences := by
-  by_contra hC;
-  sorry;
+lemma iff_eq {P : M.Predicate} : P.names M.true_sentences ↔ ∀ S : M.Sentence, (↑S ∈ P.valuated ↔ ⊨ S) := by
+  constructor;
+  . intro h S; rw [h];
+    apply Function.Injective.mem_set_image Sentence.toWord_injective;
+  . intro h;
+    sorry;
+  /-
+  simp [Predicate.names, Sentence.iff_isTrue, true_sentences];
+  constructor;
+  . intro h S;
+    replace h := subset_of_eq h;
+    constructor;
+    . intro h₂;
+      exact Function.Injective.mem_set_image Sentence.toWord_injective |>.mp $ Set.mem_of_subset_of_mem h h₂
+    . intro h₂;
+      have := @Set.mem_of_subset_of_mem (M.Word) (s₁ := P.valuated) (s₂ := M.true_sentences) (a := S.W) h;
+      sorry;
+  . intro S;
+    apply Set.eq_of_subset_of_subset;
+    . sorry;
+    . sorry;
+  -/
 
-theorem goedel1 [M.IsNR] (hP : P.valuated ⊆ M.true_sentences) : ∃ S : M.Sentence, ↑S ∉ P.valuated ∧ ↑(~S) ∈ P.valuated := by
-  by_contra hC;
-  sorry;
+lemma iff_of_names_true_sentenes {P : M.Predicate} : P.names M.true_sentences → ∀ S : M.Sentence, (↑S ∈ P.valuated ↔ ⊨ S) := by
+  intro h S; rw [h];
+  apply Function.Injective.mem_set_image Sentence.toWord_injective;
+
+theorem tarski [M.IsNR] : ∀ P : M.Predicate, ¬P.names M.true_sentences := by
+  intro P;
+  apply not_imp_not.mpr $ iff_of_names_true_sentenes;
+  apply not_forall.mpr;
+  use (~P).fixpoint;
+  rw [iff_fixpoint_is_true];
+  tauto;
+
+theorem goedel1 [M.IsNR] (hP : P.valuated ⊆ M.true_sentences) : ∃ S : M.Sentence, ↑S ∉ P.valuated ∧ ↑(~S) ∉ P.valuated := by
+  use (~P).fixpoint;
+  constructor;
+  . sorry;
+  . sorry;
 
 end SmullyanModel
